De-limited almost finished

Big_Blue_Steps.thy
@@ -37,448 +37,438 @@ definition m_of where "m_of \<equiv> \<lambda>l::nat. nat\<lceil>l powr (2/3)\<r
 context Book
 begin
 
-proposition Blue_4_1:
-  assumes "0 < \<mu>"
-  shows "\<forall>\<^sup>\<infinity>l. \<forall>k. Colours l k \<longrightarrow> 
-               (\<forall>X. X\<subseteq>V \<longrightarrow> many_bluish \<mu> l k X \<longrightarrow> 
-                    (\<exists>S T. good_blue_book \<mu> X (S,T) \<and> card S \<ge> l powr (1/4)))"
-proof -
-
-  let ?Big = "\<lambda>l. m_of l \<ge> 12  \<and>  l \<ge> (6/\<mu>) powr (12/5)  \<and>  l \<ge> 15
+definition "Big_Blue_4_1 \<equiv> 
+      \<lambda>\<mu> l. m_of l \<ge> 12  \<and>  l \<ge> (6/\<mu>) powr (12/5)  \<and>  l \<ge> 15
                \<and> 1 \<le> 5/4 * exp (- ((b_of l)^2) / ((\<mu> - 2/l) * m_of l))  \<and>  \<mu> > 2/l
                \<and> 2/l \<le> (\<mu> - 2/l) * ((5/4) powr (1/b_of l) - 1)"
-  have big_enough_l: "\<forall>\<^sup>\<infinity>l. ?Big l"
-    unfolding m_of_def b_of_def using assms by (intro eventually_conj; real_asymp)
 
-  have "\<exists>S T. good_blue_book \<mu> X (S, T) \<and> l powr (1/4) \<le> card S"
-    if big: "?Big l" and "X\<subseteq>V" and manyb: "many_bluish \<mu> l k X" and "Colours l k" for l k X
+text \<open>establishing the size requirements for 4.1\<close>
+lemma Big_Blue_4_1:
+  assumes "0<\<mu>"
+  shows "\<forall>\<^sup>\<infinity>l. Big_Blue_4_1 \<mu> l"
+  using assms
+  unfolding Big_Blue_4_1_def eventually_conj_iff m_of_def b_of_def
+  by (intro conjI eventually_all_ge_at_top; real_asymp)
+
+proposition Blue_4_1:
+  assumes "0 < \<mu>" and "Colours l k" "X\<subseteq>V" and manyb: "many_bluish \<mu> l k X"
+    and big: "Big_Blue_4_1 \<mu> l"
+  shows "\<exists>S T. good_blue_book \<mu> X (S,T) \<and> card S \<ge> l powr (1/4)"
+proof -
+  obtain ln0: "l>0" and kn0: "k>0"
+    using \<open>Colours l k\<close> Colours_kn0 Colours_ln0 by blast
+  obtain "l\<le>k" and no_Red_clique: "\<not> (\<exists>K. size_clique k K Red)" and no_Blue_clique: "\<not> (\<exists>K. size_clique l K Blue)"
+    using \<open>Colours l k\<close> by (auto simp: Colours_def)
+  have lpowr0[simp]: "0 \<le> \<lceil>l powr r\<rceil>" for r
+    by (metis ceiling_mono ceiling_zero powr_ge_pzero)
+  define b where "b \<equiv> b_of l"
+  define W where "W \<equiv> {x\<in>X. bluish \<mu> X x}"
+  define m where "m \<equiv> m_of l"
+  have "m>0" "m \<ge> 6" "m \<ge> 12" "b>0"
+    using big by (auto simp: Big_Blue_4_1_def m_def b_def b_of_def)
+  have Wbig: "card W \<ge> RN k m"
+    using manyb by (simp add: W_def m_def m_of_def many_bluish_def)
+  with Red_Blue_RN obtain U where "U \<subseteq> W" and U_m_Blue: "size_clique m U Blue"
+    by (metis W_def \<open>X \<subseteq> V\<close> mem_Collect_eq no_Red_clique subset_eq)
+  then obtain "card U = m" and "clique U Blue" and "U \<subseteq> V" "finite U"
+    by (simp add: finV finite_subset size_clique_def)
+  have "k \<le> RN m k"
+    using \<open>m\<ge>12\<close> by (simp add: RN_3plus)
+  then have "card X \<ge> l"
+    by (metis Collect_subset RN_commute W_def Wbig \<open>X\<subseteq>V\<close> card_mono order.trans finV finite_subset \<open>l\<le>k\<close>)
+  have "U \<noteq> X"
+    by (metis U_m_Blue \<open>card U = m\<close> \<open>l \<le> card X\<close> le_eq_less_or_eq no_Blue_clique size_clique_smaller)
+  then have "U \<subset> X"
+    using W_def \<open>U \<subseteq> W\<close> by blast
+  then have cardU_less_X: "card U < card X"
+    by (meson \<open>X\<subseteq>V\<close> finV finite_subset psubset_card_mono)
+  with \<open>X\<subseteq>V\<close> have cardXU: "card (X-U) = card X - card U"
+    by (meson \<open>U \<subset> X\<close> card_Diff_subset finV finite_subset psubset_imp_subset)
+  then have real_cardXU: "real (card (X-U)) = real (card X) - m"
+    using \<open>card U = m\<close> cardU_less_X by linarith
+  have [simp]: "m \<le> card X"
+    using \<open>card U = m\<close> cardU_less_X nless_le by blast
+  have lpowr23: "real l powr (2/3) \<le> real l powr 1"
+    using ln0 by (intro powr_mono) auto
+  then have "m \<le> l" "m \<le> k"
+    using \<open>l \<le> k\<close> by (auto simp: m_def m_of_def)
+  then have "m < RN k m"
+    using \<open>12 \<le> m\<close> RN_gt2 by auto
+  also have cX: "RN k m \<le> card X"
+    using manyb \<open>X\<subseteq>V\<close> by (metis Collect_subset W_def Wbig card_mono order_trans finV finite_subset)
+  finally have "card U < card X"
+    using \<open>card U = m\<close> by blast
+  text \<open>First part of (10)\<close>
+  have "card U * (\<mu> * card X - card U) = m * (\<mu> * (card X - card U)) - (1-\<mu>) * m\<^sup>2"
+    using cardU_less_X by (simp add: \<open>card U = m\<close> algebra_simps of_nat_diff numeral_2_eq_2)
+  also have "\<dots> \<le> real (card (Blue \<inter> all_edges_betw_un U (X-U)))"
   proof -
-    obtain ln0: "l>0" and kn0: "k>0"
-      using \<open>Colours l k\<close> Colours_kn0 Colours_ln0 by blast
-    obtain "l\<le>k" and no_Red_clique: "\<not> (\<exists>K. size_clique k K Red)" and no_Blue_clique: "\<not> (\<exists>K. size_clique l K Blue)"
-      using \<open>Colours l k\<close> by (auto simp: Colours_def)
-    have lpowr0[simp]: "0 \<le> \<lceil>l powr r\<rceil>" for r
-      by (metis ceiling_mono ceiling_zero powr_ge_pzero)
-    define b where "b \<equiv> b_of l"
-    define W where "W \<equiv> {x\<in>X. bluish \<mu> X x}"
-    define m where "m \<equiv> m_of l"
-    have "m>0" "m \<ge> 6" "m \<ge> 12" "b>0"
-      using big by (auto simp: m_def b_def b_of_def)
-    have Wbig: "card W \<ge> RN k m"
-      using manyb by (simp add: W_def m_def m_of_def many_bluish_def)
-    with Red_Blue_RN obtain U where "U \<subseteq> W" and U_m_Blue: "size_clique m U Blue"
-      by (metis W_def \<open>X \<subseteq> V\<close> mem_Collect_eq no_Red_clique subset_eq)
-    then obtain "card U = m" and "clique U Blue" and "U \<subseteq> V" "finite U"
-      by (simp add: finV finite_subset size_clique_def)
-    have "k \<le> RN m k"
-      using \<open>m\<ge>12\<close> by (simp add: RN_3plus)
-    then have "card X \<ge> l"
-      by (metis Collect_subset RN_commute W_def Wbig \<open>X\<subseteq>V\<close> card_mono order.trans finV finite_subset \<open>l\<le>k\<close>)
-    have "U \<noteq> X"
-      by (metis U_m_Blue \<open>card U = m\<close> \<open>l \<le> card X\<close> le_eq_less_or_eq no_Blue_clique size_clique_smaller)
-    then have "U \<subset> X"
-      using W_def \<open>U \<subseteq> W\<close> by blast
-    then have cardU_less_X: "card U < card X"
-      by (meson \<open>X\<subseteq>V\<close> finV finite_subset psubset_card_mono)
-    with \<open>X\<subseteq>V\<close> have cardXU: "card (X-U) = card X - card U"
-      by (meson \<open>U \<subset> X\<close> card_Diff_subset finV finite_subset psubset_imp_subset)
-    then have real_cardXU: "real (card (X-U)) = real (card X) - m"
-      using \<open>card U = m\<close> cardU_less_X by linarith
-    have [simp]: "m \<le> card X"
-      using \<open>card U = m\<close> cardU_less_X nless_le by blast
-    have lpowr23: "real l powr (2/3) \<le> real l powr 1"
-      using ln0 by (intro powr_mono) auto
-    then have "m \<le> l" "m \<le> k"
-      using \<open>l \<le> k\<close> by (auto simp: m_def m_of_def)
-    then have "m < RN k m"
-      using \<open>12 \<le> m\<close> RN_gt2 by auto
-    also have cX: "RN k m \<le> card X"
-      using manyb \<open>X\<subseteq>V\<close> by (metis Collect_subset W_def Wbig card_mono order_trans finV finite_subset)
-    finally have "card U < card X"
-      using \<open>card U = m\<close> by blast
-    text \<open>First part of (10)\<close>
-    have "card U * (\<mu> * card X - card U) = m * (\<mu> * (card X - card U)) - (1-\<mu>) * m\<^sup>2"
-      using cardU_less_X by (simp add: \<open>card U = m\<close> algebra_simps of_nat_diff numeral_2_eq_2)
-    also have "\<dots> \<le> real (card (Blue \<inter> all_edges_betw_un U (X-U)))"
+    have dfam: "disjoint_family_on (\<lambda>u. Blue \<inter> all_edges_betw_un {u} (X-U)) U"
+      by (auto simp: disjoint_family_on_def all_edges_betw_un_def)
+    have "\<mu> * (card X - card U) \<le> card (Blue \<inter> all_edges_betw_un {u} (X-U)) + (1-\<mu>) * m" 
+      if "u \<in> U" for u
     proof -
-      have dfam: "disjoint_family_on (\<lambda>u. Blue \<inter> all_edges_betw_un {u} (X-U)) U"
-        by (auto simp: disjoint_family_on_def all_edges_betw_un_def)
-      have "\<mu> * (card X - card U) \<le> card (Blue \<inter> all_edges_betw_un {u} (X-U)) + (1-\<mu>) * m" 
-        if "u \<in> U" for u
-      proof -
-        have NBU: "Neighbours Blue u \<inter> U = U - {u}"
-          using \<open>clique U Blue\<close> Red_Blue_all singleton_not_edge that 
-          by (force simp: Neighbours_def clique_def)
-        then have NBX_split: "(Neighbours Blue u \<inter> X) = (Neighbours Blue u \<inter> (X-U)) \<union> (U - {u})"
-          using \<open>U \<subset> X\<close> by blast
-        moreover have "Neighbours Blue u \<inter> (X-U) \<inter> (U - {u}) = {}"
-          by blast
-        ultimately have "card(Neighbours Blue u \<inter> X) = card(Neighbours Blue u \<inter> (X-U)) + (m - Suc 0)"
-          by (simp add: card_Un_disjoint finite_Neighbours \<open>finite U\<close> \<open>card U = m\<close> that)
-        then have "\<mu> * (card X) \<le> real (card (Neighbours Blue u \<inter> (X-U))) + real (m - Suc 0)"
-          using W_def \<open>U \<subseteq> W\<close> bluish_def that by force
-        then have "\<mu> * (card X - card U) 
+      have NBU: "Neighbours Blue u \<inter> U = U - {u}"
+        using \<open>clique U Blue\<close> Red_Blue_all singleton_not_edge that 
+        by (force simp: Neighbours_def clique_def)
+      then have NBX_split: "(Neighbours Blue u \<inter> X) = (Neighbours Blue u \<inter> (X-U)) \<union> (U - {u})"
+        using \<open>U \<subset> X\<close> by blast
+      moreover have "Neighbours Blue u \<inter> (X-U) \<inter> (U - {u}) = {}"
+        by blast
+      ultimately have "card(Neighbours Blue u \<inter> X) = card(Neighbours Blue u \<inter> (X-U)) + (m - Suc 0)"
+        by (simp add: card_Un_disjoint finite_Neighbours \<open>finite U\<close> \<open>card U = m\<close> that)
+      then have "\<mu> * (card X) \<le> real (card (Neighbours Blue u \<inter> (X-U))) + real (m - Suc 0)"
+        using W_def \<open>U \<subseteq> W\<close> bluish_def that by force
+      then have "\<mu> * (card X - card U) 
                 \<le> card (Neighbours Blue u \<inter> (X-U)) + real (m - Suc 0) - \<mu> *card U"
-          by (smt (verit) cardU_less_X nless_le of_nat_diff right_diff_distrib')
-        then have *: "\<mu> * (card X - card U) \<le> real (card (Neighbours Blue u \<inter> (X-U))) + (1-\<mu>)*m"
-          using assms by (simp add: \<open>card U = m\<close> left_diff_distrib)
-        have "inj_on (\<lambda>x. {u,x}) (Neighbours Blue u \<inter> X)"
-          by (simp add: doubleton_eq_iff inj_on_def)
-        moreover have "(\<lambda>x. {u,x}) ` (Neighbours Blue u \<inter> (X-U)) \<subseteq> Blue \<inter> all_edges_betw_un {u} (X-U)"
-          using Blue_E by (auto simp: Neighbours_def all_edges_betw_un_def)
-        ultimately have "card (Neighbours Blue u \<inter> (X-U)) \<le> card (Blue \<inter> all_edges_betw_un {u} (X-U))"
-          by (metis NBX_split Blue_eq card_image card_mono complete fin_edges finite_Diff finite_Int inj_on_Un)
-        with * show ?thesis
-          by auto
-      qed
-      then have "(card U) * (\<mu> * real (card X - card U))
+        by (smt (verit) cardU_less_X nless_le of_nat_diff right_diff_distrib')
+      then have *: "\<mu> * (card X - card U) \<le> real (card (Neighbours Blue u \<inter> (X-U))) + (1-\<mu>)*m"
+        using assms by (simp add: \<open>card U = m\<close> left_diff_distrib)
+      have "inj_on (\<lambda>x. {u,x}) (Neighbours Blue u \<inter> X)"
+        by (simp add: doubleton_eq_iff inj_on_def)
+      moreover have "(\<lambda>x. {u,x}) ` (Neighbours Blue u \<inter> (X-U)) \<subseteq> Blue \<inter> all_edges_betw_un {u} (X-U)"
+        using Blue_E by (auto simp: Neighbours_def all_edges_betw_un_def)
+      ultimately have "card (Neighbours Blue u \<inter> (X-U)) \<le> card (Blue \<inter> all_edges_betw_un {u} (X-U))"
+        by (metis NBX_split Blue_eq card_image card_mono complete fin_edges finite_Diff finite_Int inj_on_Un)
+      with * show ?thesis
+        by auto
+    qed
+    then have "(card U) * (\<mu> * real (card X - card U))
              \<le> (\<Sum>x\<in>U. card (Blue \<inter> all_edges_betw_un {x} (X-U)) + (1-\<mu>) * m)"
-        by (meson sum_bounded_below)
-      then have "m * (\<mu> * (card X - card U))
+      by (meson sum_bounded_below)
+    then have "m * (\<mu> * (card X - card U))
              \<le> (\<Sum>x\<in>U. card (Blue \<inter> all_edges_betw_un {x} (X-U))) + (1-\<mu>) * m\<^sup>2"
-        by (simp add: sum.distrib power2_eq_square \<open>card U = m\<close> mult_ac)
-      also have "\<dots> \<le> card (\<Union>u\<in>U. Blue \<inter> all_edges_betw_un {u} (X-U)) + (1-\<mu>) * m\<^sup>2"
-        by (simp add: dfam card_UN_disjoint' \<open>finite U\<close> flip: UN_simps)
-      finally have "m * (\<mu> * (card X - card U)) 
+      by (simp add: sum.distrib power2_eq_square \<open>card U = m\<close> mult_ac)
+    also have "\<dots> \<le> card (\<Union>u\<in>U. Blue \<inter> all_edges_betw_un {u} (X-U)) + (1-\<mu>) * m\<^sup>2"
+      by (simp add: dfam card_UN_disjoint' \<open>finite U\<close> flip: UN_simps)
+    finally have "m * (\<mu> * (card X - card U)) 
                 \<le> card (\<Union>u\<in>U. Blue \<inter> all_edges_betw_un {u} (X-U)) + (1-\<mu>) * m\<^sup>2" .
-      moreover have "(\<Union>u\<in>U. Blue \<inter> all_edges_betw_un {u} (X-U)) = (Blue \<inter> all_edges_betw_un U (X-U))"
-        by (auto simp: all_edges_betw_un_def)
-      ultimately show ?thesis
-        by simp
-    qed
-    also have "\<dots> \<le> edge_card Blue U (X-U)"
-      by (simp add: edge_card_def)
-    finally have edge_card_XU: "edge_card Blue U (X-U) \<ge> card U * (\<mu> * card X - card U)" .
-    define \<sigma> where "\<sigma> \<equiv> blue_density U (X-U)"
-    then have "\<sigma> \<ge> 0" by (simp add: gen_density_ge0)
-    have "\<sigma> \<le> 1"
-      by (simp add: \<sigma>_def gen_density_le1)
-    have 6: "real (6*k) \<le> real (2 + k*m)"
-      by (metis mult.commute \<open>12\<le>m\<close> mult_le_mono nle_le numeral_Bit0 of_nat_mono trans_le_add2)
-    then have km: "k + m \<le> Suc (k * m)"
-      using big \<open>l \<le> k\<close> \<open>m \<le> l\<close> by linarith
-    have "m/2 * (2 + real k * (1-\<mu>)) \<le> m/2 * (2 + real k)"
-      using assms by (simp add: algebra_simps)
-    also have "\<dots> \<le> (k - 1) * (m - 1)"
-      using big \<open>l \<le> k\<close> 6 \<open>m \<le> k\<close> by (simp add: algebra_simps of_nat_diff km)
-    finally  have "(m/2) * (2 + k * (1-\<mu>)) \<le> RN k m"
-      using RN_times_lower' [of k m] by linarith
-    then have "\<mu> - 2/k \<le> (\<mu> * card X - card U) / (card X - card U)"
-      using kn0 assms cardU_less_X \<open>card U = m\<close> cX by (simp add: of_nat_diff field_simps)
-    also have "\<dots> \<le> \<sigma>"
-      using \<open>m>0\<close> \<open>card U = m\<close> cardU_less_X cardXU edge_card_XU
-      by (simp add: \<sigma>_def gen_density_def field_simps mult_less_0_iff zero_less_mult_iff)
-    finally have eq10: "\<mu> - 2/k \<le> \<sigma>" .
-    have "2 * b / m \<le> \<mu> - 2/k"
-    proof -
-      have 512: "5/12 \<le> (1::real)"
-        by simp
-      with big have "l powr (5/12) \<ge> ((6/\<mu>) powr (12/5)) powr (5/12)"
-        by (simp add: powr_mono2)
-      then have lge: "l powr (5/12) \<ge> 6/\<mu>"
-        using assms powr_powr by force
-      have "2 * b \<le> 2 * (l powr (1/4) + 1)"
-        by (simp add: b_def b_of_def del: zero_le_ceiling distrib_left_numeral)
-      then have "2*b / m + 2/l \<le> 2 * (l powr (1/4) + 1) / l powr (2/3) + 2/l"
-        by (simp add: m_def m_of_def frac_le ln0 del: zero_le_ceiling distrib_left_numeral)
-      also have "\<dots> \<le> (2 * l powr (1/4) + 4) / l powr (2/3)"
-        using ln0 lpowr23 by (simp add: pos_le_divide_eq pos_divide_le_eq algebra_simps)
-      also have "\<dots> \<le> (2 * l powr (1/4) + 4 * l powr (1/4)) / l powr (2/3)"
-        using big by (simp add: divide_right_mono ge_one_powr_ge_zero)
-      also have "\<dots> = 6 / l powr (5/12)"
-        by (simp add: divide_simps flip: powr_add)
-      also have "\<dots> \<le> \<mu>"
-        using lge assms by (simp add: divide_le_eq mult.commute)
-      finally have "2*b / m + 2/l \<le> \<mu>" .
-      then show ?thesis
-        using \<open>l \<le> k\<close> \<open>m>0\<close> ln0 by (smt (verit, best) frac_le of_nat_0_less_iff of_nat_mono)
-    qed
-    with eq10 have "2 / (m/b) \<le> \<sigma>"
+    moreover have "(\<Union>u\<in>U. Blue \<inter> all_edges_betw_un {u} (X-U)) = (Blue \<inter> all_edges_betw_un U (X-U))"
+      by (auto simp: all_edges_betw_un_def)
+    ultimately show ?thesis
       by simp
-    moreover have "l powr (2/3) \<le> nat \<lceil>real l powr (2/3)\<rceil>"
-      using of_nat_ceiling by blast
-    ultimately have ble: "b \<le> \<sigma> * m / 2"
-      using mult_left_mono \<open>\<sigma> \<ge> 0\<close> big kn0 \<open>l \<le> k\<close> unfolding b_def m_def powr_diff
-      by (simp add: divide_simps)
-    then have "\<sigma> > 0"
-      using \<open>0 < b\<close> \<open>0 \<le> \<sigma>\<close> less_eq_real_def by force
-
-    define \<Phi> where "\<Phi> \<equiv> \<Sum>v \<in> X-U. card (Neighbours Blue v \<inter> U) choose b"
-    text \<open>now for the material between (10) and (11)\<close>
-    have "\<sigma> * real m / 2 \<le> m"
-      using \<open>\<sigma> \<le> 1\<close> \<open>m>0\<close> by auto
-    with ble have "b \<le> m"
-      by linarith
-    have "\<mu>^b * 1 * card X \<le> (5/4 * \<sigma>^b) * (5/4 * exp(- of_nat (b\<^sup>2) / (\<sigma>*m))) * (5/4 * (card X - m))"
-    proof (intro mult_mono)
-      have 2: "2/k \<le> 2/l"
-        by (simp add: \<open>l \<le> k\<close> frac_le ln0)
-      also have "\<dots> \<le> (\<mu> - 2/l) * ((5/4) powr (1/b) - 1)"
-        using big by (simp add: b_def)
-      also have "\<dots> \<le> \<sigma> * ((5/4) powr (1/b) - 1)"
-      proof (intro mult_right_mono)
-        show "\<mu> - 2 / real l \<le> \<sigma>"
-          using "2" eq10 by auto
-        show "0 \<le> (5/4) powr (1/b) - 1"
-          by (simp add: ge_one_powr_ge_zero)
-      qed
-      finally have "2 / real k \<le> \<sigma> * ((5/4) powr (1/b) - 1)" .
-      then have 1: "\<mu> \<le> (5/4)powr(1/b) * \<sigma>"
-        using eq10 \<open>b>0\<close> by (simp add: algebra_simps)
-      show "\<mu> ^ b \<le> 5/4 * \<sigma> ^ b"
-        using power_mono[OF 1, of b] assms \<open>\<sigma>>0\<close> \<open>b>0\<close>
-        by (simp add: powr_mult powr_powr flip: powr_realpow)
-      have "\<mu> - 2/l \<le> \<sigma>"
-        by (smt (verit, ccfv_SIG) \<open>l \<le> k\<close> eq10 frac_le ln0 of_nat_0_less_iff of_nat_mono)
-      moreover
-      have "2/l < \<mu>"
-        using big by auto
-      ultimately have "exp (- (b^2) / ((\<mu> - 2/l) * m)) \<le> exp (- real (b\<^sup>2) / (\<sigma> * real m))"
-        using \<open>\<sigma>>0\<close> \<open>m>0\<close> by (simp add: frac_le)
-      then show "1 \<le> 5/4 * exp (- of_nat (b\<^sup>2) / (\<sigma> * real m))"
-        by (smt (verit, best) b_def divide_minus_left frac_le big m_def mult_left_mono)
-      have "25 * (real m * real m) \<le> 2 powr real m"
-        using of_nat_mono [OF power2_12 [OF \<open>12 \<le> m\<close>]] by (simp add: power2_eq_square powr_realpow)
-      then have "real (5 * m) \<le>  2 powr (real m / 2)"
-        by (simp add: powr_half_sqrt_powr power2_eq_square real_le_rsqrt)
-      moreover
-      have "card X > 2 powr (m/2)"
-        by (metis RN_commute RN_lower_nodiag \<open>6 \<le> m\<close> \<open>m \<le> k\<close> add_leE less_le_trans cX numeral_Bit0 of_nat_mono)
-      ultimately have "5 * m \<le> real (card X)"
-        by linarith
-      then show "real (card X) \<le> 5/4 * real (card X - m)"
-        using \<open>card U = m\<close> cardU_less_X by simp
-    qed (use \<open>0 \<le> \<sigma>\<close> in auto)
-    also have "\<dots> \<le> 2 * (\<sigma>^b) * exp(- b\<^sup>2 / (\<sigma>*m)) * ((card X - m))"
-      by (simp add: \<open>0 \<le> \<sigma>\<close>)
-    finally have "\<mu>^b/2 * card X \<le> \<sigma>^b * exp(- of_nat (b\<^sup>2) / (\<sigma>*m)) * card (X-U)"
-      by (simp add: \<open>card U = m\<close> cardXU real_cardXU)
-    also have "\<dots> \<le> 1/(m choose b) * ((\<sigma>*m) gchoose b) * card (X-U)"
-    proof (intro mult_right_mono)
-      have "0 < real m gchoose b"
-        by (metis \<open>b \<le> m\<close> binomial_gbinomial of_nat_0_less_iff zero_less_binomial_iff)
-      then have "\<sigma> ^ b * ((real m gchoose b) * exp (- ((real b)\<^sup>2 / (\<sigma> * real m)))) \<le> \<sigma> * real m gchoose b"
-        using Fact_D1_73 [OF \<open>\<sigma>>0\<close> \<open>\<sigma>\<le>1\<close> ble] \<open>b\<le>m\<close> cardU_less_X \<open>0 < \<sigma>\<close>
-        by (simp add: field_split_simps binomial_gbinomial)
-      then show "\<sigma>^b * exp (- real (b\<^sup>2) / (\<sigma> * m)) \<le> 1/(m choose b) * (\<sigma> * m gchoose b)"
-        using \<open>b\<le>m\<close> cardU_less_X \<open>0 < \<sigma>\<close> \<open>0 < m gchoose b\<close>
-        by (simp add: field_split_simps binomial_gbinomial)
-    qed auto
-    also have "\<dots> = 1/(m choose b) * (((\<sigma>*m) gchoose b) * card (X-U))"
-      by (simp add: mult.assoc)
-    also have "\<dots> \<le> 1/(m choose b) * \<Phi>"
-    proof (intro mult_left_mono)
-      have eeq: "edge_card Blue U (X-U) = (\<Sum>i\<in>X-U. card (Neighbours Blue i \<inter> U))"
-      proof (intro edge_card_eq_sum_Neighbours)
-        show "finite (X-U)"
-          by (meson \<open>X\<subseteq>V\<close> finV finite_Diff finite_subset)
-      qed (use disjnt_def Blue_E in auto)
-      have "(\<Sum>i\<in>X - U. card (Neighbours Blue i \<inter> U)) / (real (card X) - m) = blue_density U (X-U) * m"
-        using \<open>m>0\<close> by (simp add: gen_density_def real_cardXU \<open>card U = m\<close> eeq divide_simps)
-      then have *: "(\<Sum>i\<in>X - U. real (card (Neighbours Blue i \<inter> U)) /\<^sub>R real (card (X-U))) = \<sigma> * m"
-        by (simp add: \<sigma>_def divide_inverse_commute real_cardXU flip: sum_distrib_left)
-      have "mbinomial (\<Sum>i\<in>X - U. real (card (Neighbours Blue i \<inter> U)) /\<^sub>R (card (X-U))) b 
-         \<le> (\<Sum>i\<in>X - U. inverse (real (card (X-U))) * mbinomial (card (Neighbours Blue i \<inter> U)) b)"
-      proof (rule convex_on_sum)
-        show "finite (X-U)"
-          using cardU_less_X zero_less_diff by fastforce
-        show "convex_on UNIV (\<lambda>a. mbinomial a b)"
-          by (simp add: \<open>0 < b\<close> convex_mbinomial)
-        show "(\<Sum>i\<in>X - U. inverse (card (X-U))) = 1"
-          using cardU_less_X cardXU by force
-      qed (use \<open>U \<subset> X\<close> in auto)
-      with ble 
-      show "(\<sigma>*m gchoose b) * card (X-U) \<le> \<Phi>"
-        unfolding * \<Phi>_def 
-        by (simp add: cardU_less_X cardXU binomial_gbinomial divide_simps  flip: sum_distrib_left sum_divide_distrib)
-    qed auto
-    finally have 11: "\<mu>^b / 2 * card X \<le> \<Phi> / (m choose b)"
-      by simp 
-
-    define \<Omega> where "\<Omega> \<equiv> nsets U b"  \<comment>\<open>Choose a random subset of size @{term b}\<close>
-    have card\<Omega>: "card \<Omega> = m choose b"
-      by (simp add: \<Omega>_def \<open>card U = m\<close>)
-    then have fin\<Omega>: "finite \<Omega>" and "\<Omega> \<noteq> {}" and "card \<Omega> > 0"
-      using \<open>b \<le> m\<close> not_less by fastforce+
-    define M where "M \<equiv> uniform_count_measure \<Omega>"
-    interpret P: prob_space M
-      using M_def \<open>b \<le> m\<close> card\<Omega> fin\<Omega> prob_space_uniform_count_measure by force
-    have measure_eq: "measure M C = (if C \<subseteq> \<Omega> then card C / card \<Omega> else 0)" for C
-      by (simp add: M_def fin\<Omega> measure_uniform_count_measure_if) 
-
-    define Int_NB where "Int_NB \<equiv> \<lambda>S. \<Inter>v\<in>S. Neighbours Blue v \<inter> (X-U)"
-    have sum_card_NB: "(\<Sum>A\<in>\<Omega>. card (\<Inter>(Neighbours Blue ` A) \<inter> Y)) 
-                     = (\<Sum>v\<in>Y. card (Neighbours Blue v \<inter> U) choose b)"
-      if "finite Y" "Y \<subseteq> X-U" for Y
-      using that
-    proof (induction Y)
-      case (insert y Y)
-      have *: "\<Omega> \<inter> {A. \<forall>x\<in>A. y \<in> Neighbours Blue x} = nsets (Neighbours Blue y \<inter> U) b"
-        "\<Omega> \<inter> - {A. \<forall>x\<in>A. y \<in> Neighbours Blue x} = \<Omega> - nsets (Neighbours Blue y \<inter> U) b"
-        "[Neighbours Blue y \<inter> U]\<^bsup>b\<^esup> \<subseteq> \<Omega>"
-        using insert.prems by (auto simp: \<Omega>_def nsets_def in_Neighbours_iff insert_commute)
-      then show ?case
-        using insert fin\<Omega> 
-        by (simp add: Int_insert_right sum_Suc sum.If_cases if_distrib [of card] 
-            sum.subset_diff flip: insert.IH)
-    qed auto
-
-    have "(\<Sum>x\<in>\<Omega>. card (if x = {} then UNIV else \<Inter> (Neighbours Blue ` x) \<inter> (X-U))) 
-        = (\<Sum>x\<in>\<Omega>. card (\<Inter> (Neighbours Blue ` x) \<inter> (X-U)))"
-      unfolding \<Omega>_def nsets_def using \<open>0 < b\<close> by (force intro: sum.cong)
-    also have "\<dots> = (\<Sum>v\<in>X - U. card (Neighbours Blue v \<inter> U) choose b)"
-      by (metis sum_card_NB \<open>X\<subseteq>V\<close> dual_order.refl finV finite_Diff rev_finite_subset)
-    finally have "sum (card o Int_NB) \<Omega> = \<Phi>"
-      by (simp add: \<Omega>_def \<Phi>_def Int_NB_def)
-    moreover
-    have "ennreal (P.expectation (\<lambda>S. card (Int_NB S))) = sum (card o Int_NB) \<Omega> / (card \<Omega>)"
-      using integral_uniform_count_measure M_def fin\<Omega> by fastforce
-    ultimately have P: "P.expectation (\<lambda>S. card (Int_NB S)) = \<Phi> / (m choose b)"
-      by (metis Bochner_Integration.integral_nonneg card\<Omega> divide_nonneg_nonneg ennreal_inj of_nat_0_le_iff)
-    have False if "\<And>S. S \<in> \<Omega> \<Longrightarrow> card (Int_NB S) < \<Phi> / (m choose b)"
-    proof -
-      define L where "L \<equiv> (\<lambda>S. \<Phi> / real (m choose b) - card (Int_NB S)) ` \<Omega>"
-      have "finite L" "L \<noteq> {}"
-        using L_def fin\<Omega>  \<open>\<Omega>\<noteq>{}\<close> by blast+
-      define \<epsilon> where "\<epsilon> \<equiv> Min L"
-      have "\<epsilon> > 0"
-        using that fin\<Omega> \<open>\<Omega> \<noteq> {}\<close> by (simp add: L_def \<epsilon>_def)
-      then have "\<And>S. S \<in> \<Omega> \<Longrightarrow> card (Int_NB S) \<le> \<Phi> / (m choose b) - \<epsilon>"
-        using linorder_class.Min_le [OF \<open>finite L\<close>]
-        by (fastforce simp add: algebra_simps \<epsilon>_def L_def)
-      then have "P.expectation (\<lambda>S. card (Int_NB S)) \<le> \<Phi> / (m choose b) - \<epsilon>"
-        using P P.not_empty not_integrable_integral_eq \<open>\<epsilon> > 0\<close>
-        by (intro P.integral_le_const) (fastforce simp: M_def space_uniform_count_measure)+
-      then show False
-        using P \<open>0 < \<epsilon>\<close> by auto
-    qed
-    then obtain S where "S \<in> \<Omega>" and Sge: "card (Int_NB S) \<ge> \<Phi> / (m choose b)"
-      using linorder_not_le by blast
-    then have "S \<subseteq> U"
-      by (simp add: \<Omega>_def nsets_def subset_iff)
-    have "card S = b" "clique S Blue"
-      using \<open>S \<in> \<Omega>\<close> \<open>U \<subseteq> V\<close> \<open>clique U Blue\<close> smaller_clique 
-      unfolding \<Omega>_def nsets_def size_clique_def by auto
-    have "\<Phi> / (m choose b) \<ge> \<mu>^b * card X / 2"
-      using 11 by simp
-    then have S: "card (Int_NB S) \<ge> \<mu>^b * card X / 2"
-      using Sge by linarith
-    obtain v where "v \<in> S"
-      using \<open>0 < b\<close> \<open>card S = b\<close> by fastforce
-    have "all_edges_betw_un S (S \<union> Int_NB S) \<subseteq> Blue"
-      using \<open>clique S Blue\<close> unfolding all_edges_betw_un_def Neighbours_def clique_def Int_NB_def
-      by fastforce
-    then have "good_blue_book \<mu> X (S, Int_NB S)"
-      using \<open>S\<subseteq>U\<close> \<open>v \<in> S\<close> \<open>U \<subset> X\<close> S \<open>card S = b\<close>
-      unfolding good_blue_book_def book_def size_clique_def Int_NB_def disjnt_iff
-      by blast
-    then show ?thesis
-      by (metis \<open>card S = b\<close> b_def b_of_def of_nat_ceiling)
   qed
-  with eventually_mono [OF big_enough_l] show ?thesis
-    by presburger 
-qed
+  also have "\<dots> \<le> edge_card Blue U (X-U)"
+    by (simp add: edge_card_def)
+  finally have edge_card_XU: "edge_card Blue U (X-U) \<ge> card U * (\<mu> * card X - card U)" .
+  define \<sigma> where "\<sigma> \<equiv> blue_density U (X-U)"
+  then have "\<sigma> \<ge> 0" by (simp add: gen_density_ge0)
+  have "\<sigma> \<le> 1"
+    by (simp add: \<sigma>_def gen_density_le1)
+  have 6: "real (6*k) \<le> real (2 + k*m)"
+    by (metis mult.commute \<open>12\<le>m\<close> mult_le_mono nle_le numeral_Bit0 of_nat_mono trans_le_add2)
+  then have km: "k + m \<le> Suc (k * m)"
+    using big \<open>l \<le> k\<close> \<open>m \<le> l\<close> by linarith
+  have "m/2 * (2 + real k * (1-\<mu>)) \<le> m/2 * (2 + real k)"
+    using assms by (simp add: algebra_simps)
+  also have "\<dots> \<le> (k - 1) * (m - 1)"
+    using big \<open>l \<le> k\<close> 6 \<open>m \<le> k\<close> by (simp add: Big_Blue_4_1_def algebra_simps of_nat_diff km)
+  finally  have "(m/2) * (2 + k * (1-\<mu>)) \<le> RN k m"
+    using RN_times_lower' [of k m] by linarith
+  then have "\<mu> - 2/k \<le> (\<mu> * card X - card U) / (card X - card U)"
+    using kn0 assms cardU_less_X \<open>card U = m\<close> cX by (simp add: of_nat_diff field_simps)
+  also have "\<dots> \<le> \<sigma>"
+    using \<open>m>0\<close> \<open>card U = m\<close> cardU_less_X cardXU edge_card_XU
+    by (simp add: \<sigma>_def gen_density_def field_simps mult_less_0_iff zero_less_mult_iff)
+  finally have eq10: "\<mu> - 2/k \<le> \<sigma>" .
+  have "2 * b / m \<le> \<mu> - 2/k"
+  proof -
+    have 512: "5/12 \<le> (1::real)"
+      by simp
+    with big have "l powr (5/12) \<ge> ((6/\<mu>) powr (12/5)) powr (5/12)"
+      by (simp add: Big_Blue_4_1_def powr_mono2)
+    then have lge: "l powr (5/12) \<ge> 6/\<mu>"
+      using assms powr_powr by force
+    have "2 * b \<le> 2 * (l powr (1/4) + 1)"
+      by (simp add: b_def b_of_def del: zero_le_ceiling distrib_left_numeral)
+    then have "2*b / m + 2/l \<le> 2 * (l powr (1/4) + 1) / l powr (2/3) + 2/l"
+      by (simp add: m_def m_of_def frac_le ln0 del: zero_le_ceiling distrib_left_numeral)
+    also have "\<dots> \<le> (2 * l powr (1/4) + 4) / l powr (2/3)"
+      using ln0 lpowr23 by (simp add: pos_le_divide_eq pos_divide_le_eq algebra_simps)
+    also have "\<dots> \<le> (2 * l powr (1/4) + 4 * l powr (1/4)) / l powr (2/3)"
+      using big by (simp add: Big_Blue_4_1_def divide_right_mono ge_one_powr_ge_zero)
+    also have "\<dots> = 6 / l powr (5/12)"
+      by (simp add: divide_simps flip: powr_add)
+    also have "\<dots> \<le> \<mu>"
+      using lge assms by (simp add: divide_le_eq mult.commute)
+    finally have "2*b / m + 2/l \<le> \<mu>" .
+    then show ?thesis
+      using \<open>l \<le> k\<close> \<open>m>0\<close> ln0 by (smt (verit, best) frac_le of_nat_0_less_iff of_nat_mono)
+  qed
+  with eq10 have "2 / (m/b) \<le> \<sigma>"
+    by simp
+  moreover have "l powr (2/3) \<le> nat \<lceil>real l powr (2/3)\<rceil>"
+    using of_nat_ceiling by blast
+  ultimately have ble: "b \<le> \<sigma> * m / 2"
+    using mult_left_mono \<open>\<sigma> \<ge> 0\<close> big kn0 \<open>l \<le> k\<close> 
+    by (simp add: Big_Blue_4_1_def powr_diff b_def m_def divide_simps)
+  then have "\<sigma> > 0"
+    using \<open>0 < b\<close> \<open>0 \<le> \<sigma>\<close> less_eq_real_def by force
 
-definition "Lemma_bblue_step_limit \<equiv> \<lambda>\<mu> l. \<forall>k. Colours l k \<longrightarrow> card (Step_class \<mu> l k {bblue_step}) \<le> l powr (3/4)"
+  define \<Phi> where "\<Phi> \<equiv> \<Sum>v \<in> X-U. card (Neighbours Blue v \<inter> U) choose b"
+  text \<open>now for the material between (10) and (11)\<close>
+  have "\<sigma> * real m / 2 \<le> m"
+    using \<open>\<sigma> \<le> 1\<close> \<open>m>0\<close> by auto
+  with ble have "b \<le> m"
+    by linarith
+  have "\<mu>^b * 1 * card X \<le> (5/4 * \<sigma>^b) * (5/4 * exp(- of_nat (b\<^sup>2) / (\<sigma>*m))) * (5/4 * (card X - m))"
+  proof (intro mult_mono)
+    have 2: "2/k \<le> 2/l"
+      by (simp add: \<open>l \<le> k\<close> frac_le ln0)
+    also have "\<dots> \<le> (\<mu> - 2/l) * ((5/4) powr (1/b) - 1)"
+      using big by (simp add: Big_Blue_4_1_def b_def)
+    also have "\<dots> \<le> \<sigma> * ((5/4) powr (1/b) - 1)"
+    proof (intro mult_right_mono)
+      show "\<mu> - 2 / real l \<le> \<sigma>"
+        using "2" eq10 by auto
+      show "0 \<le> (5/4) powr (1/b) - 1"
+        by (simp add: ge_one_powr_ge_zero)
+    qed
+    finally have "2 / real k \<le> \<sigma> * ((5/4) powr (1/b) - 1)" .
+    then have 1: "\<mu> \<le> (5/4)powr(1/b) * \<sigma>"
+      using eq10 \<open>b>0\<close> by (simp add: algebra_simps)
+    show "\<mu> ^ b \<le> 5/4 * \<sigma> ^ b"
+      using power_mono[OF 1, of b] assms \<open>\<sigma>>0\<close> \<open>b>0\<close>
+      by (simp add: powr_mult powr_powr flip: powr_realpow)
+    have "\<mu> - 2/l \<le> \<sigma>"
+      by (smt (verit, ccfv_SIG) \<open>l \<le> k\<close> eq10 frac_le ln0 of_nat_0_less_iff of_nat_mono)
+    moreover have "2/l < \<mu>"
+      using big by (auto simp: Big_Blue_4_1_def) 
+    ultimately have "exp (- (b^2) / ((\<mu> - 2/l) * m)) \<le> exp (- real (b\<^sup>2) / (\<sigma> * real m))"
+      using \<open>\<sigma>>0\<close> \<open>m>0\<close> by (simp add: frac_le)
+    then show "1 \<le> 5/4 * exp (- of_nat (b\<^sup>2) / (\<sigma> * real m))"
+      using big unfolding Big_Blue_4_1_def b_def m_def
+      by (smt (verit, best) divide_minus_left frac_le mult_left_mono)
+    have "25 * (real m * real m) \<le> 2 powr real m"
+      using of_nat_mono [OF power2_12 [OF \<open>12 \<le> m\<close>]] by (simp add: power2_eq_square powr_realpow)
+    then have "real (5 * m) \<le>  2 powr (real m / 2)"
+      by (simp add: powr_half_sqrt_powr power2_eq_square real_le_rsqrt)
+    moreover
+    have "card X > 2 powr (m/2)"
+      by (metis RN_commute RN_lower_nodiag \<open>6 \<le> m\<close> \<open>m \<le> k\<close> add_leE less_le_trans cX numeral_Bit0 of_nat_mono)
+    ultimately have "5 * m \<le> real (card X)"
+      by linarith
+    then show "real (card X) \<le> 5/4 * real (card X - m)"
+      using \<open>card U = m\<close> cardU_less_X by simp
+  qed (use \<open>0 \<le> \<sigma>\<close> in auto)
+  also have "\<dots> \<le> 2 * (\<sigma>^b) * exp(- b\<^sup>2 / (\<sigma>*m)) * ((card X - m))"
+    by (simp add: \<open>0 \<le> \<sigma>\<close>)
+  finally have "\<mu>^b/2 * card X \<le> \<sigma>^b * exp(- of_nat (b\<^sup>2) / (\<sigma>*m)) * card (X-U)"
+    by (simp add: \<open>card U = m\<close> cardXU real_cardXU)
+  also have "\<dots> \<le> 1/(m choose b) * ((\<sigma>*m) gchoose b) * card (X-U)"
+  proof (intro mult_right_mono)
+    have "0 < real m gchoose b"
+      by (metis \<open>b \<le> m\<close> binomial_gbinomial of_nat_0_less_iff zero_less_binomial_iff)
+    then have "\<sigma> ^ b * ((real m gchoose b) * exp (- ((real b)\<^sup>2 / (\<sigma> * real m)))) \<le> \<sigma> * real m gchoose b"
+      using Fact_D1_73 [OF \<open>\<sigma>>0\<close> \<open>\<sigma>\<le>1\<close> ble] \<open>b\<le>m\<close> cardU_less_X \<open>0 < \<sigma>\<close>
+      by (simp add: field_split_simps binomial_gbinomial)
+    then show "\<sigma>^b * exp (- real (b\<^sup>2) / (\<sigma> * m)) \<le> 1/(m choose b) * (\<sigma> * m gchoose b)"
+      using \<open>b\<le>m\<close> cardU_less_X \<open>0 < \<sigma>\<close> \<open>0 < m gchoose b\<close>
+      by (simp add: field_split_simps binomial_gbinomial)
+  qed auto
+  also have "\<dots> = 1/(m choose b) * (((\<sigma>*m) gchoose b) * card (X-U))"
+    by (simp add: mult.assoc)
+  also have "\<dots> \<le> 1/(m choose b) * \<Phi>"
+  proof (intro mult_left_mono)
+    have eeq: "edge_card Blue U (X-U) = (\<Sum>i\<in>X-U. card (Neighbours Blue i \<inter> U))"
+    proof (intro edge_card_eq_sum_Neighbours)
+      show "finite (X-U)"
+        by (meson \<open>X\<subseteq>V\<close> finV finite_Diff finite_subset)
+    qed (use disjnt_def Blue_E in auto)
+    have "(\<Sum>i\<in>X - U. card (Neighbours Blue i \<inter> U)) / (real (card X) - m) = blue_density U (X-U) * m"
+      using \<open>m>0\<close> by (simp add: gen_density_def real_cardXU \<open>card U = m\<close> eeq divide_simps)
+    then have *: "(\<Sum>i\<in>X - U. real (card (Neighbours Blue i \<inter> U)) /\<^sub>R real (card (X-U))) = \<sigma> * m"
+      by (simp add: \<sigma>_def divide_inverse_commute real_cardXU flip: sum_distrib_left)
+    have "mbinomial (\<Sum>i\<in>X - U. real (card (Neighbours Blue i \<inter> U)) /\<^sub>R (card (X-U))) b 
+         \<le> (\<Sum>i\<in>X - U. inverse (real (card (X-U))) * mbinomial (card (Neighbours Blue i \<inter> U)) b)"
+    proof (rule convex_on_sum)
+      show "finite (X-U)"
+        using cardU_less_X zero_less_diff by fastforce
+      show "convex_on UNIV (\<lambda>a. mbinomial a b)"
+        by (simp add: \<open>0 < b\<close> convex_mbinomial)
+      show "(\<Sum>i\<in>X - U. inverse (card (X-U))) = 1"
+        using cardU_less_X cardXU by force
+    qed (use \<open>U \<subset> X\<close> in auto)
+    with ble 
+    show "(\<sigma>*m gchoose b) * card (X-U) \<le> \<Phi>"
+      unfolding * \<Phi>_def 
+      by (simp add: cardU_less_X cardXU binomial_gbinomial divide_simps  flip: sum_distrib_left sum_divide_distrib)
+  qed auto
+  finally have 11: "\<mu>^b / 2 * card X \<le> \<Phi> / (m choose b)"
+    by simp 
+
+  define \<Omega> where "\<Omega> \<equiv> nsets U b"  \<comment>\<open>Choose a random subset of size @{term b}\<close>
+  have card\<Omega>: "card \<Omega> = m choose b"
+    by (simp add: \<Omega>_def \<open>card U = m\<close>)
+  then have fin\<Omega>: "finite \<Omega>" and "\<Omega> \<noteq> {}" and "card \<Omega> > 0"
+    using \<open>b \<le> m\<close> not_less by fastforce+
+  define M where "M \<equiv> uniform_count_measure \<Omega>"
+  interpret P: prob_space M
+    using M_def \<open>b \<le> m\<close> card\<Omega> fin\<Omega> prob_space_uniform_count_measure by force
+  have measure_eq: "measure M C = (if C \<subseteq> \<Omega> then card C / card \<Omega> else 0)" for C
+    by (simp add: M_def fin\<Omega> measure_uniform_count_measure_if) 
+
+  define Int_NB where "Int_NB \<equiv> \<lambda>S. \<Inter>v\<in>S. Neighbours Blue v \<inter> (X-U)"
+  have sum_card_NB: "(\<Sum>A\<in>\<Omega>. card (\<Inter>(Neighbours Blue ` A) \<inter> Y)) 
+                     = (\<Sum>v\<in>Y. card (Neighbours Blue v \<inter> U) choose b)"
+    if "finite Y" "Y \<subseteq> X-U" for Y
+    using that
+  proof (induction Y)
+    case (insert y Y)
+    have *: "\<Omega> \<inter> {A. \<forall>x\<in>A. y \<in> Neighbours Blue x} = nsets (Neighbours Blue y \<inter> U) b"
+      "\<Omega> \<inter> - {A. \<forall>x\<in>A. y \<in> Neighbours Blue x} = \<Omega> - nsets (Neighbours Blue y \<inter> U) b"
+      "[Neighbours Blue y \<inter> U]\<^bsup>b\<^esup> \<subseteq> \<Omega>"
+      using insert.prems by (auto simp: \<Omega>_def nsets_def in_Neighbours_iff insert_commute)
+    then show ?case
+      using insert fin\<Omega> 
+      by (simp add: Int_insert_right sum_Suc sum.If_cases if_distrib [of card] 
+          sum.subset_diff flip: insert.IH)
+  qed auto
+
+  have "(\<Sum>x\<in>\<Omega>. card (if x = {} then UNIV else \<Inter> (Neighbours Blue ` x) \<inter> (X-U))) 
+        = (\<Sum>x\<in>\<Omega>. card (\<Inter> (Neighbours Blue ` x) \<inter> (X-U)))"
+    unfolding \<Omega>_def nsets_def using \<open>0 < b\<close> by (force intro: sum.cong)
+  also have "\<dots> = (\<Sum>v\<in>X - U. card (Neighbours Blue v \<inter> U) choose b)"
+    by (metis sum_card_NB \<open>X\<subseteq>V\<close> dual_order.refl finV finite_Diff rev_finite_subset)
+  finally have "sum (card o Int_NB) \<Omega> = \<Phi>"
+    by (simp add: \<Omega>_def \<Phi>_def Int_NB_def)
+  moreover
+  have "ennreal (P.expectation (\<lambda>S. card (Int_NB S))) = sum (card o Int_NB) \<Omega> / (card \<Omega>)"
+    using integral_uniform_count_measure M_def fin\<Omega> by fastforce
+  ultimately have P: "P.expectation (\<lambda>S. card (Int_NB S)) = \<Phi> / (m choose b)"
+    by (metis Bochner_Integration.integral_nonneg card\<Omega> divide_nonneg_nonneg ennreal_inj of_nat_0_le_iff)
+  have False if "\<And>S. S \<in> \<Omega> \<Longrightarrow> card (Int_NB S) < \<Phi> / (m choose b)"
+  proof -
+    define L where "L \<equiv> (\<lambda>S. \<Phi> / real (m choose b) - card (Int_NB S)) ` \<Omega>"
+    have "finite L" "L \<noteq> {}"
+      using L_def fin\<Omega>  \<open>\<Omega>\<noteq>{}\<close> by blast+
+    define \<epsilon> where "\<epsilon> \<equiv> Min L"
+    have "\<epsilon> > 0"
+      using that fin\<Omega> \<open>\<Omega> \<noteq> {}\<close> by (simp add: L_def \<epsilon>_def)
+    then have "\<And>S. S \<in> \<Omega> \<Longrightarrow> card (Int_NB S) \<le> \<Phi> / (m choose b) - \<epsilon>"
+      using linorder_class.Min_le [OF \<open>finite L\<close>]
+      by (fastforce simp add: algebra_simps \<epsilon>_def L_def)
+    then have "P.expectation (\<lambda>S. card (Int_NB S)) \<le> \<Phi> / (m choose b) - \<epsilon>"
+      using P P.not_empty not_integrable_integral_eq \<open>\<epsilon> > 0\<close>
+      by (intro P.integral_le_const) (fastforce simp: M_def space_uniform_count_measure)+
+    then show False
+      using P \<open>0 < \<epsilon>\<close> by auto
+  qed
+  then obtain S where "S \<in> \<Omega>" and Sge: "card (Int_NB S) \<ge> \<Phi> / (m choose b)"
+    using linorder_not_le by blast
+  then have "S \<subseteq> U"
+    by (simp add: \<Omega>_def nsets_def subset_iff)
+  have "card S = b" "clique S Blue"
+    using \<open>S \<in> \<Omega>\<close> \<open>U \<subseteq> V\<close> \<open>clique U Blue\<close> smaller_clique 
+    unfolding \<Omega>_def nsets_def size_clique_def by auto
+  have "\<Phi> / (m choose b) \<ge> \<mu>^b * card X / 2"
+    using 11 by simp
+  then have S: "card (Int_NB S) \<ge> \<mu>^b * card X / 2"
+    using Sge by linarith
+  obtain v where "v \<in> S"
+    using \<open>0 < b\<close> \<open>card S = b\<close> by fastforce
+  have "all_edges_betw_un S (S \<union> Int_NB S) \<subseteq> Blue"
+    using \<open>clique S Blue\<close> unfolding all_edges_betw_un_def Neighbours_def clique_def Int_NB_def
+    by fastforce
+  then have "good_blue_book \<mu> X (S, Int_NB S)"
+    using \<open>S\<subseteq>U\<close> \<open>v \<in> S\<close> \<open>U \<subset> X\<close> S \<open>card S = b\<close>
+    unfolding good_blue_book_def book_def size_clique_def Int_NB_def disjnt_iff
+    by blast
+  then show ?thesis
+    by (metis \<open>card S = b\<close> b_def b_of_def of_nat_ceiling)
+qed
 
 text \<open>Lemma 4.3\<close>
 proposition bblue_step_limit:
-  assumes "\<mu>>0"
-  shows "\<forall>\<^sup>\<infinity>l. Lemma_bblue_step_limit \<mu> l"
+  assumes "\<mu>>0" and "Colours l k" and big: "Big_Blue_4_1 \<mu> l"
+  shows "card (Step_class \<mu> l k {bblue_step}) \<le> l powr (3/4)"
 proof -
-  have "card (Step_class \<mu> l k {bblue_step}) \<le> l powr (3/4)"
-    if 41: "\<And>X. many_bluish \<mu> l k X \<Longrightarrow> X\<subseteq>V \<Longrightarrow> \<exists>S T. good_blue_book \<mu> X (S,T) \<and> card S \<ge> l powr (1/4)"
-      and "Colours l k" for l k
-  proof -
-    define BBLUES where "BBLUES \<equiv> \<lambda>r. {m. m < r \<and> stepper_kind \<mu> l k m = bblue_step}"
-    have cardB_ge: "card B \<ge> b_of l * card(BBLUES n)"
-      if "stepper \<mu> l k n = (X,Y,A,B)" for n X Y A B
-      using that
-    proof (induction n arbitrary: X Y A B)
-      case 0 then show ?case by (auto simp: BBLUES_def)
+  define BBLUES where "BBLUES \<equiv> \<lambda>r. {m. m < r \<and> stepper_kind \<mu> l k m = bblue_step}"
+  have cardB_ge: "card B \<ge> b_of l * card(BBLUES n)"
+    if "stepper \<mu> l k n = (X,Y,A,B)" for n X Y A B
+    using that
+  proof (induction n arbitrary: X Y A B)
+    case 0 then show ?case by (auto simp: BBLUES_def)
+  next
+    case (Suc n)
+    obtain X' Y' A' B' where step_n: "stepper \<mu> l k n = (X',Y',A',B')"
+      by (metis surj_pair)
+    then have "valid_state (X',Y',A',B')"
+      by (metis valid_state_stepper)
+    have "B' \<subseteq> B"
+      using Suc by (auto simp: next_state_def Let_def degree_reg_def step_n split: prod.split_asm if_split_asm)
+    show ?case
+    proof (cases "stepper_kind \<mu> l k n = bblue_step")
+      case True
+      have [simp]: "card (insert n (BBLUES n)) = Suc (card (BBLUES n))"
+        by (simp add: BBLUES_def)
+      have card_B': "card B' \<ge> b_of l * card (BBLUES n)"
+        using step_n BBLUES_def Suc.IH by blast
+      obtain S where "A' = A" "Y' = Y" and manyb: "many_bluish \<mu> l k X'" 
+        and cbb: "choose_blue_book \<mu> (X',Y,A,B') = (S,X)" and le_cardB: "card (B' \<union> S) \<le> card B"
+        using Suc.prems True
+        by (auto simp: stepper_kind_def next_state_kind_def next_state_def step_n split: prod.split_asm if_split_asm)     
+      then have VS: "V_state (X',Y,A,B')" and ds: "disjoint_state (X',Y,A,B')"
+        using \<open>valid_state (X',Y',A',B')\<close> by (auto simp: valid_state_def)
+      then obtain "X' \<subseteq> V" "finite X'"
+        by (metis Xseq_subset_V finX step_n stepper_XYseq)
+      then have l14: "l powr (1/4) \<le> real (card S)"
+        using \<open>Colours l k\<close> Blue_4_1 [OF \<open>\<mu>>0\<close> \<open>Colours l k\<close> _ manyb big]
+        by (smt (verit, best) best_blue_book_is_best cbb choose_blue_book_works of_nat_mono)
+      then have ble: "b_of l \<le> card S"
+        using b_of_def nat_ceiling_le_eq by presburger
+      have S: "good_blue_book \<mu> X' (S,X)"
+        by (metis choose_blue_book_works \<open>finite X'\<close> cbb)
+      have "card S \<le> best_blue_book_card \<mu> X'"
+        using S \<open>finite X'\<close> best_blue_book_is_best by blast
+      have fin: "finite B'" "finite S"
+        using Colours_ln0 \<open>Colours l k\<close> l14 VS finB by force+
+      have "disjnt B' S"
+        using ds S by (force simp: disjoint_state_def good_blue_book_def disjnt_iff)
+      have eq: "BBLUES(Suc n) = insert n (BBLUES n)"
+        using less_Suc_eq True unfolding BBLUES_def by blast
+      then have "b_of l * card (BBLUES (Suc n)) = b_of l + b_of l * card (BBLUES n)"
+        by auto
+      also have "\<dots> \<le> card B' + card S"
+        using ble card_B' by linarith
+      also have "... \<le> card (B' \<union> S)"
+        using ble \<open>disjnt B' S\<close> fin by (simp add: card_Un_disjnt)
+      finally have **: "b_of l * card (BBLUES (Suc n)) \<le> card B"
+        using dual_order.trans le_cardB by blast 
+      then show ?thesis
+        by (simp add: BBLUES_def)
     next
-      case (Suc n)
-      obtain X' Y' A' B' where step_n: "stepper \<mu> l k n = (X',Y',A',B')"
-        by (metis surj_pair)
-      then have "valid_state (X',Y',A',B')"
-        by (metis valid_state_stepper)
-      have "B' \<subseteq> B"
-        using Suc by (auto simp: next_state_def Let_def degree_reg_def step_n split: prod.split_asm if_split_asm)
-      show ?case
-      proof (cases "stepper_kind \<mu> l k n = bblue_step")
-        case True
-        have [simp]: "card (insert n (BBLUES n)) = Suc (card (BBLUES n))"
-          by (simp add: BBLUES_def)
-        have card_B': "card B' \<ge> b_of l * card (BBLUES n)"
-          using step_n BBLUES_def Suc.IH by blast
-        obtain S where "A' = A" "Y' = Y" and manyb: "many_bluish \<mu> l k X'" 
-          and cbb: "choose_blue_book \<mu> (X',Y,A,B') = (S,X)" and le_cardB: "card (B' \<union> S) \<le> card B"
-          using Suc.prems True
-          by (auto simp: stepper_kind_def next_state_kind_def next_state_def step_n split: prod.split_asm if_split_asm)     
-        then have VS: "V_state (X',Y,A,B')" and ds: "disjoint_state (X',Y,A,B')"
-          using \<open>valid_state (X',Y',A',B')\<close> by (auto simp: valid_state_def)
-        then obtain "X' \<subseteq> V" "finite X'"
-          by (metis Xseq_subset_V finX step_n stepper_XYseq)
-        then have l14: "l powr (1/4) \<le> real (card S)"
-          using \<open>Colours l k\<close> 41 [OF manyb] 
-          by (smt (verit, best) best_blue_book_is_best cbb choose_blue_book_works of_nat_mono)
-        then have ble: "b_of l \<le> card S"
-          using b_of_def nat_ceiling_le_eq by presburger
-        have S: "good_blue_book \<mu> X' (S,X)"
-          by (metis choose_blue_book_works \<open>finite X'\<close> cbb)
-        have "card S \<le> best_blue_book_card \<mu> X'"
-          using S \<open>finite X'\<close> best_blue_book_is_best by blast
-        have fin: "finite B'" "finite S"
-          using Colours_ln0 \<open>Colours l k\<close> l14 VS finB by force+
-        have "disjnt B' S"
-          using ds S by (force simp: disjoint_state_def good_blue_book_def disjnt_iff)
-        have eq: "BBLUES(Suc n) = insert n (BBLUES n)"
-          using less_Suc_eq True unfolding BBLUES_def by blast
-        then have "b_of l * card (BBLUES (Suc n)) = b_of l + b_of l * card (BBLUES n)"
-          by auto
-        also have "\<dots> \<le> card B' + card S"
-          using ble card_B' by linarith
-        also have "... \<le> card (B' \<union> S)"
-          using ble \<open>disjnt B' S\<close> fin by (simp add: card_Un_disjnt)
-        finally have **: "b_of l * card (BBLUES (Suc n)) \<le> card B"
-          using dual_order.trans le_cardB by blast 
-        then show ?thesis
-          by (simp add: BBLUES_def)
-      next
-        case False
-        then have "BBLUES(Suc n) = BBLUES n"
-          using less_Suc_eq by (auto simp: BBLUES_def) 
-        with \<open>B' \<subseteq> B\<close> show ?thesis
-          by (metis Suc V_state_stepper card_mono dual_order.trans finB step_n)
-      qed
+      case False
+      then have "BBLUES(Suc n) = BBLUES n"
+        using less_Suc_eq by (auto simp: BBLUES_def) 
+      with \<open>B' \<subseteq> B\<close> show ?thesis
+        by (metis Suc V_state_stepper card_mono dual_order.trans finB step_n)
     qed
-    { assume \<section>: "card (Step_class \<mu> l k {bblue_step}) > l powr (3/4)"
-      then have fin: "finite (Step_class \<mu> l k {bblue_step})"
-        using card.infinite by fastforce
-      then obtain n where n: "(Step_class \<mu> l k {bblue_step}) = {m. m<n \<and> stepper_kind \<mu> l k m = bblue_step}"
-        using Step_class_iterates by blast
-      with \<section> have card_gt: "card{m. m<n \<and> stepper_kind \<mu> l k m = bblue_step} > l powr (3/4)"
-        by (simp add: n)
-      obtain X Y A B where step: "stepper \<mu> l k n = (X,Y,A,B)"
-        using prod_cases4 by blast
-      have "l = l powr (1/4) * l powr (3/4)"
-        by (simp flip: powr_add)
-      also have "\<dots> \<le> b_of l * l powr (3/4)"
-        by (simp add: b_of_def mult_mono')
-      also have "\<dots> \<le> b_of l * card{m. m<n \<and> stepper_kind \<mu> l k m = bblue_step}"
-        using card_gt less_eq_real_def by fastforce
-      also have "... \<le> card B"
-        using cardB_ge step of_nat_mono unfolding BBLUES_def by blast
-      also have "... < l"
-        using stepper_B[OF step] \<open>\<mu>>0\<close> \<open>Colours l k\<close>
-        by (metis Colours_def linorder_neqE_nat of_nat_less_iff size_clique_def size_clique_smaller)
-      finally have False
-        by simp
-    } 
-    then show ?thesis by force
   qed
-  with eventually_mono [OF Blue_4_1] \<open>\<mu>>0\<close> show ?thesis
-    unfolding Lemma_bblue_step_limit_def by presburger 
+  { assume \<section>: "card (Step_class \<mu> l k {bblue_step}) > l powr (3/4)"
+    then have fin: "finite (Step_class \<mu> l k {bblue_step})"
+      using card.infinite by fastforce
+    then obtain n where n: "(Step_class \<mu> l k {bblue_step}) = {m. m<n \<and> stepper_kind \<mu> l k m = bblue_step}"
+      using Step_class_iterates by blast
+    with \<section> have card_gt: "card{m. m<n \<and> stepper_kind \<mu> l k m = bblue_step} > l powr (3/4)"
+      by (simp add: n)
+    obtain X Y A B where step: "stepper \<mu> l k n = (X,Y,A,B)"
+      using prod_cases4 by blast
+    have "l = l powr (1/4) * l powr (3/4)"
+      by (simp flip: powr_add)
+    also have "\<dots> \<le> b_of l * l powr (3/4)"
+      by (simp add: b_of_def mult_mono')
+    also have "\<dots> \<le> b_of l * card{m. m<n \<and> stepper_kind \<mu> l k m = bblue_step}"
+      using card_gt less_eq_real_def by fastforce
+    also have "... \<le> card B"
+      using cardB_ge step of_nat_mono unfolding BBLUES_def by blast
+    also have "... < l"
+      using stepper_B[OF step] \<open>\<mu>>0\<close> \<open>Colours l k\<close>
+      by (metis Colours_def linorder_neqE_nat of_nat_less_iff size_clique_def size_clique_smaller)
+    finally have False
+      by simp
+  } 
+  then show ?thesis by force
 qed
 
 proposition red_step_limit:
@@ -550,132 +540,119 @@ proof -
     unfolding REDS_def by (metis (mono_tags) Step_class_iterates [OF red_step_finite [OF assms]] )
 qed
 
-definition 
-  "Lemma_bblue_dboost_step_limit \<equiv> 
-     \<lambda>\<mu> l. \<forall>k. Colours l k \<longrightarrow>
-     card (Step_class \<mu> l k {bblue_step}) + card (Step_class \<mu> l k {dboost_step}) < l"
-
 proposition bblue_dboost_step_limit:
-  assumes "\<mu>>0"
-  shows "\<forall>\<^sup>\<infinity>l. Lemma_bblue_dboost_step_limit \<mu> l"
+  assumes "\<mu>>0" and "Colours l k" and big: "Big_Blue_4_1 \<mu> l"
+  shows "card (Step_class \<mu> l k {bblue_step}) + card (Step_class \<mu> l k {dboost_step}) < l"
 proof -
-  have "card (Step_class \<mu> l k {bblue_step}) + card (Step_class \<mu> l k {dboost_step}) < l"
-    if 41: "\<And>X. many_bluish \<mu> l k X \<Longrightarrow> X\<subseteq>V \<Longrightarrow> \<exists>S T. good_blue_book \<mu> X (S,T) \<and> card S \<ge> l powr (1/4)"
-      and "Colours l k" for l k
-  proof -
-    define BDB where "BDB \<equiv> \<lambda>r. {m. m < r \<and> stepper_kind \<mu> l k m \<in> {bblue_step,dboost_step}}"
-    have *: "card(BDB n) \<le> card B"
-      if "stepper \<mu> l k n = (X,Y,A,B)" for n X Y A B
-      using that
-    proof (induction n arbitrary: X Y A B)
-      case 0
-      then show ?case
+  define BDB where "BDB \<equiv> \<lambda>r. {m. m < r \<and> stepper_kind \<mu> l k m \<in> {bblue_step,dboost_step}}"
+  have *: "card(BDB n) \<le> card B"
+    if "stepper \<mu> l k n = (X,Y,A,B)" for n X Y A B
+    using that
+  proof (induction n arbitrary: X Y A B)
+    case 0
+    then show ?case
+      by (auto simp: BDB_def)
+  next
+    case (Suc n)
+    obtain X' Y' A' B' where step_n: "stepper \<mu> l k n = (X',Y',A',B')"
+      by (metis surj_pair)
+    then obtain "valid_state (X',Y',A',B')" and "V_state (X',Y',A',B')"
+      and disjst: "disjoint_state(X',Y',A',B')" and "finite X'"
+      by (metis finX valid_state_def valid_state_stepper)
+    have "B' \<subseteq> B"
+      using Suc.prems by (auto simp: next_state_def Let_def degree_reg_def step_n split: prod.split_asm if_split_asm)
+    show ?case
+    proof (cases "stepper_kind \<mu> l k n \<in> {bblue_step,dboost_step}")
+      case True
+      then have "BDB (Suc n) = insert n (BDB n)"
         by (auto simp: BDB_def)
-    next
-      case (Suc n)
-      obtain X' Y' A' B' where step_n: "stepper \<mu> l k n = (X',Y',A',B')"
-        by (metis surj_pair)
-      then obtain "valid_state (X',Y',A',B')" and "V_state (X',Y',A',B')"
-        and disjst: "disjoint_state(X',Y',A',B')" and "finite X'"
-        by (metis finX valid_state_def valid_state_stepper)
-      have "B' \<subseteq> B"
-        using Suc.prems by (auto simp: next_state_def Let_def degree_reg_def step_n split: prod.split_asm if_split_asm)
-      show ?case
-      proof (cases "stepper_kind \<mu> l k n \<in> {bblue_step,dboost_step}")
-        case True
-        then have "BDB (Suc n) = insert n (BDB n)"
-          by (auto simp: BDB_def)
-        moreover have "card (insert n (BDB n)) = Suc (card (BDB n))"
-          by (simp add: BDB_def)
-        ultimately have card_Suc[simp]: "card (BDB (Suc n)) = Suc (card (BDB n))"
-          by presburger
-        have card_B': "card (BDB n) \<le> card B'"
-          using step_n BDB_def Suc.IH by blast
-        consider "stepper_kind \<mu> l k n = bblue_step" | "stepper_kind \<mu> l k n = dboost_step"
-          using True by force
-        then have Bigger: "B' \<subset> B"
-        proof cases
-          case 1
-          then have "\<not> termination_condition l k X' Y'"
-            by (auto simp: stepper_kind_def step_n)
-          with 1 obtain S where "A' = A" "Y' = Y" and manyb: "many_bluish \<mu> l k X'" 
-            and cbb: "choose_blue_book \<mu> (X',Y,A,B') = (S,X)" and le_cardB: "B = B' \<union> S"
-            using Suc.prems 
-            by (auto simp: stepper_kind_def next_state_kind_def next_state_def step_n split: prod.split_asm if_split_asm)
-          then have VS: "V_state (X',Y,A,B')" and ds: "disjoint_state (X',Y,A,B')"
-            using \<open>valid_state (X',Y',A',B')\<close> by (auto simp: valid_state_def)
-          then obtain "X' \<subseteq> V" "finite X'"
-            by (metis Xseq_subset_V finX step_n stepper_XYseq)
-          then have "l powr (1/4) \<le> real (card S)"
-            using \<open>Colours l k\<close> 41 [OF manyb]
-            by (smt (verit, best) VS best_blue_book_is_best cbb choose_blue_book_works of_nat_mono)
-          then have "S \<noteq> {}"
-            using Colours_ln0 \<open>Colours l k\<close> by fastforce
-          moreover have "disjnt B' S"
-            using choose_blue_book_subset [OF \<open>finite X'\<close>] disjst cbb
-            unfolding disjoint_state_def
-            by (smt (verit) in_mono \<open>A' = A\<close> \<open>Y' = Y\<close> disjnt_iff old.prod.case)
-          ultimately show ?thesis
-            by (metis \<open>B' \<subseteq> B\<close> disjnt_Un1 disjnt_self_iff_empty le_cardB psubsetI)
-        next
-          case 2
-          then have "choose_central_vx \<mu> (X',Y',A',B') \<in> X'"
-            unfolding stepper_kind_def next_state_kind_def 
-            by (auto simp: \<open>finite X'\<close> choose_central_vx_X step_n split: if_split_asm)
-          moreover have "disjnt B' X'"
-            using disjst disjnt_sym by (force simp add: disjoint_state_def)
-          ultimately have "choose_central_vx \<mu> (X',Y',A',B') \<notin> B'"
-            by (meson disjnt_iff)
-          then show ?thesis
-            using 2 Suc.prems 
-            by (auto simp: stepper_kind_def next_state_kind_def next_state_def step_n Let_def split: if_split_asm)
-        qed
-        moreover have "finite B"
-          by (metis Suc.prems V_state_stepper finB)
+      moreover have "card (insert n (BDB n)) = Suc (card (BDB n))"
+        by (simp add: BDB_def)
+      ultimately have card_Suc[simp]: "card (BDB (Suc n)) = Suc (card (BDB n))"
+        by presburger
+      have card_B': "card (BDB n) \<le> card B'"
+        using step_n BDB_def Suc.IH by blast
+      consider "stepper_kind \<mu> l k n = bblue_step" | "stepper_kind \<mu> l k n = dboost_step"
+        using True by force
+      then have Bigger: "B' \<subset> B"
+      proof cases
+        case 1
+        then have "\<not> termination_condition l k X' Y'"
+          by (auto simp: stepper_kind_def step_n)
+        with 1 obtain S where "A' = A" "Y' = Y" and manyb: "many_bluish \<mu> l k X'" 
+          and cbb: "choose_blue_book \<mu> (X',Y,A,B') = (S,X)" and le_cardB: "B = B' \<union> S"
+          using Suc.prems 
+          by (auto simp: stepper_kind_def next_state_kind_def next_state_def step_n split: prod.split_asm if_split_asm)
+        then have VS: "V_state (X',Y,A,B')" and ds: "disjoint_state (X',Y,A,B')"
+          using \<open>valid_state (X',Y',A',B')\<close> by (auto simp: valid_state_def)
+        then obtain "X' \<subseteq> V" "finite X'"
+          by (metis Xseq_subset_V finX step_n stepper_XYseq)
+        then have "l powr (1/4) \<le> real (card S)"
+        using \<open>Colours l k\<close> Blue_4_1 [OF \<open>\<mu>>0\<close> \<open>Colours l k\<close> _ manyb big]
+          by (smt (verit, best) VS best_blue_book_is_best cbb choose_blue_book_works of_nat_mono)
+        then have "S \<noteq> {}"
+          using Colours_ln0 \<open>Colours l k\<close> by fastforce
+        moreover have "disjnt B' S"
+          using choose_blue_book_subset [OF \<open>finite X'\<close>] disjst cbb
+          unfolding disjoint_state_def
+          by (smt (verit) in_mono \<open>A' = A\<close> \<open>Y' = Y\<close> disjnt_iff old.prod.case)
         ultimately show ?thesis
-          by (metis card_B' card_Suc card_seteq le_trans not_less_eq_eq psubset_eq)
+          by (metis \<open>B' \<subseteq> B\<close> disjnt_Un1 disjnt_self_iff_empty le_cardB psubsetI)
       next
-        case False
-        then have "BDB (Suc n) = BDB n"
-          using less_Suc_eq unfolding BDB_def by blast
-        with \<open>B' \<subseteq> B\<close> show ?thesis
-          by (smt (verit, best) Suc V_state_stepper card_seteq order.trans finB nat_le_linear step_n)
+        case 2
+        then have "choose_central_vx \<mu> (X',Y',A',B') \<in> X'"
+          unfolding stepper_kind_def next_state_kind_def 
+          by (auto simp: \<open>finite X'\<close> choose_central_vx_X step_n split: if_split_asm)
+        moreover have "disjnt B' X'"
+          using disjst disjnt_sym by (force simp add: disjoint_state_def)
+        ultimately have "choose_central_vx \<mu> (X',Y',A',B') \<notin> B'"
+          by (meson disjnt_iff)
+        then show ?thesis
+          using 2 Suc.prems 
+          by (auto simp: step_kind_defs next_state_def step_n Let_def split: if_split_asm)
       qed
+      moreover have "finite B"
+        by (metis Suc.prems V_state_stepper finB)
+      ultimately show ?thesis
+        by (metis card_B' card_Suc card_seteq le_trans not_less_eq_eq psubset_eq)
+    next
+      case False
+      then have "BDB (Suc n) = BDB n"
+        using less_Suc_eq unfolding BDB_def by blast
+      with \<open>B' \<subseteq> B\<close> show ?thesis
+        by (smt (verit, best) Suc V_state_stepper card_seteq order.trans finB nat_le_linear step_n)
     qed
-    have less_l: "card (BDB n) < l" for n
-    proof -
-      obtain X Y A B where "stepper \<mu> l k n = (X,Y,A,B)"
-        using prod_cases4 by blast
-      with * show ?thesis
-        using \<open>Colours l k\<close> card_B_limit by fastforce
-    qed
-    moreover have fin: "\<And>n. finite (BDB n)" "incseq BDB"
-      by (auto simp: BDB_def incseq_def)
-    ultimately have **: "\<forall>\<^sup>\<infinity>n. \<Union> (range BDB) = BDB n"
-      using Union_incseq_finite by blast
-    then have "finite (\<Union> (range BDB))"
-      using BDB_def eventually_sequentially by force
-    moreover have Uneq: "\<Union> (range BDB) = Step_class \<mu> l k {bblue_step,dboost_step}"
-      by (auto simp: Step_class_def BDB_def)
-    ultimately have fin: "finite (Step_class \<mu> l k {bblue_step,dboost_step})"
-      by fastforce
-    obtain n where "\<Union> (range BDB) = BDB n"
-      using ** by force
-    then have "card (BDB n) = card (Step_class \<mu> l k {bblue_step} \<union> Step_class \<mu> l k {dboost_step})"
-      by (metis Step_class_insert Uneq)
-    also have "\<dots> = card (Step_class \<mu> l k {bblue_step}) + card (Step_class \<mu> l k {dboost_step})"
-    proof -
-      have "disjnt (Step_class \<mu> l k {bblue_step}) (Step_class \<mu> l k {dboost_step})"
-        using disjnt_Step_class by auto
-      then show ?thesis
-        using fin dboost_step_finite [OF assms]
-        by (metis Step_class_insert card_Un_disjnt finite_Un)
-    qed
-    finally show ?thesis
-      by (metis less_l)
   qed
-  with eventually_mono [OF Blue_4_1] \<open>\<mu>>0\<close> show ?thesis
-    unfolding Lemma_bblue_dboost_step_limit_def by presburger 
+  have less_l: "card (BDB n) < l" for n
+  proof -
+    obtain X Y A B where "stepper \<mu> l k n = (X,Y,A,B)"
+      using prod_cases4 by blast
+    with * show ?thesis
+      using \<open>Colours l k\<close> card_B_limit by fastforce
+  qed
+  moreover have fin: "\<And>n. finite (BDB n)" "incseq BDB"
+    by (auto simp: BDB_def incseq_def)
+  ultimately have **: "\<forall>\<^sup>\<infinity>n. \<Union> (range BDB) = BDB n"
+    using Union_incseq_finite by blast
+  then have "finite (\<Union> (range BDB))"
+    using BDB_def eventually_sequentially by force
+  moreover have Uneq: "\<Union> (range BDB) = Step_class \<mu> l k {bblue_step,dboost_step}"
+    by (auto simp: Step_class_def BDB_def)
+  ultimately have fin: "finite (Step_class \<mu> l k {bblue_step,dboost_step})"
+    by fastforce
+  obtain n where "\<Union> (range BDB) = BDB n"
+    using ** by force
+  then have "card (BDB n) = card (Step_class \<mu> l k {bblue_step} \<union> Step_class \<mu> l k {dboost_step})"
+    by (metis Step_class_insert Uneq)
+  also have "\<dots> = card (Step_class \<mu> l k {bblue_step}) + card (Step_class \<mu> l k {dboost_step})"
+  proof -
+    have "disjnt (Step_class \<mu> l k {bblue_step}) (Step_class \<mu> l k {dboost_step})"
+      using disjnt_Step_class by auto
+    then show ?thesis
+      by (metis Step_class_insert card_Un_disjnt fin finite_Un)
+  qed
+  finally show ?thesis
+    by (metis less_l)
 qed
 
 end
